# 4.2
$$
\begin{align*}
&\mathbb{P}\{X_n = j | X_{n_1} = i_1, \cdots, X_{n_k} = i_k\} \\
&= \sum_{x_{n_k+1},x_{n_k+2} \cdots x_{n-1}} \mathbb{P}\{X_n = j, X_{n-1} = x_{n-1}, \cdots, X_{n_k+1} = x_{n_k+1} | X_{n_1} = i_1, \cdots, X_{n_k} = i_k\} \\
&= \sum_{x_{n_k+1},x_{n_k+2}} \mathbb{P}\{X_n = j | X_{n-1} = x_{n-1}\} \mathbb{P}\{X_{n-1} = x_{n-1} | X_{n-2} = x_{n-2}\} \\&\cdots \mathbb{P}\{X_{n_k+1} = x_{n_k+1} | X_{n_k} = i_k\} \\
&= \mathbb{P}\{X_n = j | X_{n_k} = i_k\}
\end{align*}
$$

---

# 4.8
